src/impl/TLS13.Impl.Driver.Pairing.fsti
@@ -488,6 +488,15 @@ let client_server_driver_supported_profile_derived_projection_inputs
   client_server_driver_x25519_projection_inputs client server /\
   client_server_driver_application_derivation_projection_inputs client server
 
+noextract
+let client_server_driver_supported_profile_derived_key_share_projection_inputs
+  (client:CS.connection_state)
+  (server:CS.connection_state)
+  : prop =
+  client_server_driver_x25519_key_share_projection_inputs client server /\
+  CS.same_key_derivation_checkpoint CS.DeriveHandshakeTraffic client server /\
+  client_server_driver_application_derivation_projection_inputs client server
+
 val lemma_client_server_driver_paired_x25519_key_shares_from_projection_inputs
   (client:CS.connection_state)
   (server:CS.connection_state)
@@ -514,12 +523,35 @@ val lemma_client_server_driver_paired_key_derivation_checkpoints_from_projection
           server)
       (ensures CS.paired_key_derivation_checkpoints client server)
 
+val lemma_client_server_driver_paired_key_derivation_checkpoints_from_key_share_projection_inputs
+  (client:CS.connection_state)
+  (server:CS.connection_state)
+  : Lemma
+      (requires
+        client_server_driver_supported_profile_derived_key_share_projection_inputs
+          client
+          server)
+      (ensures CS.paired_key_derivation_checkpoints client server)
+
 val lemma_client_server_driver_supported_profile_derived_state_inputs_from_projection_inputs
   (client:CS.connection_state)
   (server:CS.connection_state)
   : Lemma
       (requires
         client_server_driver_supported_profile_derived_projection_inputs
+          client
+          server)
+      (ensures
+        client_server_driver_supported_profile_derived_state_inputs
+          client
+          server)
+
+val lemma_client_server_driver_supported_profile_derived_state_inputs_from_key_share_projection_inputs
+  (client:CS.connection_state)
+  (server:CS.connection_state)
+  : Lemma
+      (requires
+        client_server_driver_supported_profile_derived_key_share_projection_inputs
           client
           server)
       (ensures
